denotational/Vectors.v
@@ -1,0 +1,31 @@
+From Coq Require Import
+     Vector
+     Program.Equality.
+
+From Coq Require Fin.
+
+Import VectorNotations.
+From Equations Require Import Equations.
+
+From DSL Require Import Agent.
+
+Module VectorUtils.
+
+  Definition vec n T := Vector.t T n.
+
+  Definition fin := Fin.t.
+
+  Import Fin.
+  Equations vector_remove{A n}(v: vec (S n) A)(i: fin (S n)) : vec n A by wf n lt :=
+    vector_remove (h :: h' :: ts) (FS (FS j)) := h :: (vector_remove (h' :: ts) (FS j));
+    vector_remove (h :: h' :: ts) (FS F1) := h :: ts;
+    vector_remove (h :: h' :: ts) F1 := h' :: ts;
+    vector_remove (h::nil) F1 := @nil A.
+                                                   
+  Equations vector_replace{A n}(v: vec (S n) A)(i: fin (S n))(a: A): vec (S n) A by wf n lt :=
+    vector_replace (h :: h' :: ts) (FS (FS j)) a := h :: (vector_replace (h' :: ts) (FS j) a);
+    vector_replace (h :: h' :: ts) (FS F1) a := h :: a :: ts;
+    vector_replace (h :: h' :: ts) F1 a := a :: h' :: ts;
+    vector_replace (h::nil) F1 a := [a].
+
+End VectorUtils.
